Improved translation of example, Goals now take target lists
Improved the translation of the example Resolute to Coq by changing Goals to take lists of Target IDs rather than a single Target ID. This enables multivariable functions like the binding between processes and processors to be implemented correctly.

src/Resolute_Logic.v
@@ -53,7 +53,7 @@ Fixpoint appraise (e:Evidence) : AppEvidence :=
 Inductive Resolute : Type :=
   | R_False
   | R_True
-  | R_Goal (T : Target_ID) (F : Target_ID -> Resolute)
+  | R_Goal (l : list Target_ID) (F : list Target_ID -> Resolute)
   | R_And (G1 : Resolute) (G2 : Resolute)
   | R_Or (G1 : Resolute) (G2 : Resolute)
   | R_Imp (G1 : Resolute) (G2 : Resolute)
@@ -64,8 +64,8 @@ Definition Assumption := Resolute.
 Definition Assumptions := list (Assumption).
 
 Record Model := {
-  conc : Target_ID -> Term ;
-  spec : Target_ID -> list AppEvidence
+  conc : list Target_ID -> Term ;
+  spec : list Target_ID -> list AppEvidence
 }.
 
 Fixpoint res_to_copland (M : Model) (r:Resolute) : Term * (AppEvidence -> Prop) :=
@@ -74,7 +74,7 @@ Fixpoint res_to_copland (M : Model) (r:Resolute) : Term * (AppEvidence -> Prop) 
 
   | R_True => (emptyTerm, fun e => True)
 
-  | (R_Goal tid NONSENSE_PLACEHOLDER_VARIABLE_PLEASE_FIX) => (conc M tid, fun e => In e (spec M tid))
+  | (R_Goal tid fid) => (conc M tid, fun e => In e (spec M tid))
 
   | R_And r1 r2 => 
     let '(t1, pol1) := res_to_copland M r1 in
@@ -151,20 +151,22 @@ Definition targets := [1; 2; 3].
 
 Definition ex_forall := 
 R_Forall targets 
-(fun target => R_Goal target (fun target => R_True)).
+(fun target => R_Goal [target] (fun target => R_True)).
 
 Definition processes := [1; 2; 3].
 Definition processors := [1; 2; 3].
 
-Definition is_more_than_zero (T: Target_ID) : Resolute :=
-  match T with
-  | O => R_False
-  | S x => R_True
+Definition is_more_than_zero (l: list Target_ID) : Resolute :=
+  match l with
+  | [O] => R_False
+  | [S x] => R_True
+  | _ => R_False
   end.
 
-Definition is_bound (T : Target_ID) : Resolute :=
-  match T with
-  | _ => R_True
+Definition is_bound (l : list Target_ID) : Resolute :=
+  match l with
+  | [process; processor] => R_True
+  | _ => R_False 
   end.
 
 (*
@@ -180,14 +182,22 @@ R_And
   (fun process => 
     (R_Exists processors
       (fun processor =>
-        R_Goal processor is_bound
+        R_Goal [process; processor] is_bound
       )
     )
   )
 )
-(R_Goal (length processes) is_more_than_zero).
+(R_Goal ([length processes]) is_more_than_zero).
+ 
+Definition test_model := {| 
+  conc := fun _ => emptyTerm;
+  spec := fun _ => nil
+|}.
+Definition copland_one_process := res_to_copland test_model one_process.
 
-Example test_one_process : Reval nil one_process.
+Compute copland_one_process.
+
+Example test_one_process : Reval [] one_process.
 Proof.
 unfold one_process. apply Reval_And_R.
 - apply Reval_Forall. 
@@ -218,8 +228,8 @@ Proof.
     implies that an arbitrary goal can be evaluated in Reval.
     It is not clear to me yet how to use the hypothesis in this way. 
     *)
-    + intros. specialize H with (t := conc m T).
-    simpl in H. specialize H with (pol := fun e => In e (spec m T)).
+    + intros. specialize H with (t := conc m l).
+    simpl in H. specialize H with (pol := fun e => In e (spec m l)).
     simpl in H. intros. admit.
     (* Reval_And: in progress *)
     + intros. apply Reval_And_R.
